State the adequacy and upto thread composition

src/lang/Configuration.v
@@ -13,21 +13,50 @@ Require Import Thread.
 Set Implicit Arguments.
 
 
-Module Configuration.
+Module Threads.
   Definition syntax := IdentMap.t {lang:Language.t & lang.(Language.syntax)}.
+  Definition t := IdentMap.t {lang:Language.t & Thread.t lang}.
 
+  Definition init (s:syntax): t :=
+    IdentMap.map (fun s => existT _ _ (Thread.init _ s.(projT2))) s.
+
+  Definition singleton tid lang th: t :=
+    IdentMap.add tid (existT _ lang th) (IdentMap.empty _).
+
+  Definition is_terminal (ths:t): Prop :=
+    forall tid lang th (FIND: IdentMap.find tid ths = Some (existT _ lang th)),
+      Thread.is_terminal th.
+
+  Definition wf (ths:t): Prop :=
+    forall tid1 lang1 th1
+      tid2 lang2 th2
+      (TID: tid1 <> tid2)
+      (TH1: IdentMap.find tid1 ths = Some (existT _ lang1 th1))
+      (TH2: IdentMap.find tid2 ths = Some (existT _ lang2 th2)),
+      Memory.disjoint th1.(Thread.local) th2.(Thread.local).
+
+  Definition disjoint (ths1 ths2:t): Prop :=
+    forall tid1 lang1 th1
+      tid2 lang2 th2
+      (TH1: IdentMap.find tid1 ths1 = Some (existT _ lang1 th1))
+      (TH2: IdentMap.find tid2 ths2 = Some (existT _ lang2 th2)),
+      Memory.disjoint th1.(Thread.local) th2.(Thread.local).
+
+  Definition le (ths:t) (mem:Memory.t): Prop :=
+    forall tid lang th
+      (TH: IdentMap.find tid ths = Some (existT _ lang th)),
+      Memory.le th.(Thread.local) mem.
+End Threads.
+
+
+Module Configuration.
   Structure t := mk {
-    threads: IdentMap.t {lang:Language.t & Thread.t lang};
+    threads: Threads.t;
     memory: Memory.t;
   }.
 
-  Definition init (s:syntax): t :=
-    mk (IdentMap.map (fun s => existT _ _ (Thread.init _ s.(projT2))) s)
-       Memory.init.
-
-  Definition is_terminal (conf:t): Prop :=
-    forall tid lang st (FIND: IdentMap.find tid conf.(threads) = Some (existT _ lang st)),
-      Thread.is_terminal st.
+  Definition init (s:Threads.syntax): t := mk (Threads.init s) Memory.init.
+  Definition is_terminal (conf:t): Prop := Threads.is_terminal conf.(threads).
 
   Inductive step (e:option Event.t) (c1:t): forall (c2:t), Prop :=
   | step_intro
