src/opt/Simulation.v
@@ -76,3 +76,77 @@ Section SimulationThread.
   Definition sim_thread: SIM_THREAD := paco5 _sim_thread bot5.
 End SimulationThread.
 Hint Resolve _sim_thread_mon: paco.
+
+
+Section Simulation.
+  Definition SIM :=
+    forall (th1_src:Threads.t) (mem_k_src:Memory.t)
+      (th1_tgt:Threads.t) (mem_k_tgt:Memory.t), Prop.
+
+  (* TODO: inftau & liveness *)
+  Definition _sim
+             (sim: SIM)
+             (ths1_src:Threads.t) (mem_k_src:Memory.t)
+             (ths1_tgt:Threads.t) (mem_k_tgt:Memory.t): Prop :=
+    forall mem1_src mem1_tgt
+      (MEMORY1: sim_memory mem1_src mem1_tgt)
+      (LOCAL_SRC: Threads.le ths1_src mem1_src)
+      (LOCAL_TGT: Threads.le ths1_tgt mem1_tgt)
+      (FUTURE_SRC: Memory.future mem_k_src mem1_src)
+      (FUTURE_TGT: Memory.future mem_k_tgt mem1_tgt),
+      <<TERMINAL:
+        forall (TERMINAL_TGT: Threads.is_terminal ths1_tgt),
+        exists ths2_src mem2_src,
+          <<STEPS: rtc (Configuration.step None) (Configuration.mk ths1_src mem1_src) (Configuration.mk ths2_src mem2_src)>> /\
+          <<MEMORY: sim_memory mem2_src mem1_tgt>> /\
+          <<TERMINAL_SRC: Threads.is_terminal ths2_src>>>> /\
+      <<CONSISTENT:
+        forall (CONSISTENT_TGT: Configuration.consistent (Configuration.mk ths1_tgt mem1_tgt)),
+        <<CONSISTENT_SRC: Configuration.consistent (Configuration.mk ths1_src mem1_src)>>>> /\
+      <<STEP:
+        forall e ths3_tgt mem3_tgt
+          (STEP_TGT: Configuration.step e (Configuration.mk ths1_tgt mem1_tgt) (Configuration.mk ths3_tgt mem3_tgt)),
+        exists ths2_src mem2_src ths3_src mem3_src,
+          <<STEPS: rtc (Configuration.step None) (Configuration.mk ths1_src mem1_src) (Configuration.mk ths2_src mem2_src)>> /\
+          <<STEP_SRC: Configuration.step e (Configuration.mk ths2_src mem2_src) (Configuration.mk ths3_src mem3_src)>> /\
+          <<MEMORY2: sim_memory mem3_src mem3_tgt>> /\
+          <<SIM: sim ths3_src mem3_src ths3_tgt mem3_tgt>>>>.
+
+  Lemma _sim_mon: monotone4 _sim.
+  Proof.
+    ii. exploit IN; eauto. i. des.
+    splits; eauto. i.
+    exploit STEP; eauto. i. des.
+    eexists _, _, _, _. splits; eauto.
+  Qed.
+  Hint Resolve _sim_mon: paco.
+
+  Definition sim: SIM := paco4 _sim bot4.
+End Simulation.
+Hint Resolve _sim_mon: paco.
+
+
+Lemma sim_thread_sim
+      lang sim_terminal th1_src mem_k_src th1_tgt mem_k_tgt tid
+      (SIM: @sim_thread lang sim_terminal th1_src mem_k_src th1_tgt mem_k_tgt):
+  sim
+    (Threads.singleton tid th1_src) mem_k_src
+    (Threads.singleton tid th1_tgt) mem_k_tgt.
+Proof.
+  revert th1_src mem_k_src th1_tgt mem_k_tgt SIM. pcofix CIH. i.
+  punfold SIM0. pfold. ii.
+  exploit SIM0; eauto.
+  { eapply LOCAL_SRC.
+    unfold Threads.singleton. rewrite IdentMap.Facts.add_eq_o; eauto.
+  }
+  { eapply LOCAL_TGT.
+    unfold Threads.singleton. rewrite IdentMap.Facts.add_eq_o; eauto.
+  }
+  i. des. splits.
+  - i. exploit TERMINAL; eauto.
+    { admit. }
+    i. des.
+    admit.
+  - admit.
+  - admit.
+Admitted.
