src/lang/Behavior.v
@@ -1,0 +1,26 @@
+Require Import sflib.
+Require Import paco.
+
+Require Import Basic.
+Require Import Event.
+Require Import Language.
+Require Import Memory.
+Require Import Thread.
+Require Import Configuration.
+Require Import Simulation.
+
+Set Implicit Arguments.
+
+(* NOTE: we serialize all the events within a behavior, but it may not
+ * be the case.  The *NIX kernels are re-entrant: system calls may
+ * race.
+ *)
+CoInductive behavior :=
+| behvaior_nil
+| behavior_event (e:Event.t) (b:behavior)
+| behavior_inftau
+.
+
+(* TODO *)
+Definition behaviors (conf:Configuration.t) (b:behavior): Prop :=
+  False.
