src/opt/Adequacy.v
@@ -1,0 +1,20 @@
+Require Import sflib.
+Require Import paco.
+
+Require Import Basic.
+Require Import Event.
+Require Import Language.
+Require Import Memory.
+Require Import Thread.
+Require Import Configuration.
+Require Import Simulation.
+Require Import Behavior.
+
+Lemma sim_adequacy
+      ths_src mem_src
+      ths_tgt mem_tgt
+      (SIM: sim ths_src mem_src ths_tgt mem_tgt):
+  behaviors (Configuration.mk ths_src mem_src) <1=
+  behaviors (Configuration.mk ths_tgt mem_tgt).
+Proof.
+Admitted.
